src/localdrf/LocalDRFDef.v
@@ -1,0 +1,118 @@
+Require Import RelationClasses.
+
+From Paco Require Import paco.
+From sflib Require Import sflib.
+
+From PromisingLib Require Import Axioms.
+From PromisingLib Require Import Basic.
+From PromisingLib Require Import DataStructure.
+From PromisingLib Require Import Language.
+From PromisingLib Require Import Loc.
+Require Import Time.
+Require Import Event.
+Require Import View.
+Require Import Cell.
+Require Import Memory.
+Require Import MemoryFacts.
+Require Import TView.
+Require Import Local.
+Require Import Thread.
+Require Import Configuration.
+Require Import Progress.
+Require Import Behavior.
+Require Import Cover.
+Require Import Pred.
+Require Import Trace.
+
+Set Implicit Arguments.
+
+
+Inductive step_all A B C D (step: A -> B -> C -> D -> Prop): C -> D -> Prop :=
+| step_all_intro
+    a b c d
+    (STEP: step a b c d)
+  :
+    step_all step c d.
+
+Section LOCALDRF.
+
+  Variable L: Loc.t -> bool.
+
+  Definition valid_event (e: ThreadEvent.t): Prop :=
+    forall loc from to msg kind (PROMISE: e = ThreadEvent.promise loc from to msg kind) (LOC: L loc),
+      msg = Message.reserve.
+
+  Definition valid_step (e: MachineEvent.t) (tid: Ident.t)
+             (c0 c1: Configuration.t): Prop :=
+    exists lang tr,
+      (<<STEP: @Trace.configuration_step lang tr e tid c0 c1>>) /\
+      (<<VALID: List.Forall (compose valid_event snd) tr>>).
+
+  Inductive configuration_steps_trace:
+    forall (c0 c1: Configuration.t) (tr: list (Ident.t * sigT Trace.t)), Prop :=
+  | configuration_steps_trace_nil
+      c0
+    :
+      configuration_steps_trace c0 c0 []
+  | configuration_steps_trace_cons
+      c0 c1 c2 trs lang tr e tid
+      (STEPS: configuration_steps_trace c0 c1 trs)
+      (STEP: @Trace.configuration_step lang tr e tid c0 c1)
+      (VALID: List.Forall (compose valid_event snd) tr)
+    :
+      configuration_steps_trace c0 c2 (trs ++ [(tid, existT _ _ tr)]) (* add at "last" *)
+  .
+
+  Inductive racy_read (loc: Loc.t) (ts: Time.t):
+    forall lang (th: Thread.t lang) (e: ThreadEvent.t), Prop :=
+  | racy_read_read
+      lang (th: Thread.t lang)
+      valr releasedr ordr
+      (VIEW: Time.lt (th.(Thread.local).(Local.tview).(TView.cur).(View.rlx) loc) ts)
+    :
+      racy_read loc ts th (ThreadEvent.read loc ts valr releasedr ordr)
+  | racy_read_update
+      lang (th: Thread.t lang)
+      to valr valw releasedr releasedw ordr ordw
+      (VIEW: Time.lt (th.(Thread.local).(Local.tview).(TView.cur).(View.rlx) loc) ts)
+    :
+      racy_read loc ts th (ThreadEvent.update loc ts to valr valw releasedr releasedw ordr ordw)
+  .
+
+  Inductive racy_write (loc: Loc.t) (ts: Time.t):
+    forall lang (th: Thread.t lang) (e: ThreadEvent.t), Prop :=
+  | racy_write_write
+      lang (th: Thread.t lang)
+      from valw releasedw ordw
+      (ORD: Ordering.le ordw Ordering.relaxed)
+    :
+      racy_write loc ts th (ThreadEvent.write loc from ts valw releasedw ordw)
+  | racy_write_update
+      lang (th: Thread.t lang)
+      from valr valw releasedr releasedw ordr ordw
+      (ORD: Ordering.le ordw Ordering.relaxed)
+    :
+      racy_write loc ts th (ThreadEvent.update loc from ts valr valw releasedr releasedw ordr ordw)
+  .
+
+  Definition racefree (s: Threads.syntax): Prop :=
+    forall c0 c1 trs
+           loc ts
+           tid0 tid1 lang0 lang1 tr0 tr1 th0 th1 e0 e1
+           (CSTEPS: configuration_steps_trace c0 c1 trs)
+           (TRACE0: List.In (tid0, existT _ lang0 tr0) trs)
+           (TRACE1: List.In (tid1, existT _ lang1 tr1) trs)
+           (EVENT0: List.In (th0, e0) tr0)
+           (EVENT1: List.In (th1, e1) tr1)
+           (WRITE: racy_write loc ts th0 e0)
+           (READ: racy_read loc ts th1 e1),
+      False.
+
+  Theorem local_DRF_PF s
+          (RACEFRFEE: racefree s)
+    :
+      behaviors Configuration.step (Configuration.init s) <1=
+      behaviors valid_step (Configuration.init s).
+  Admitted.
+
+End LOCALDRF.
